Some more work

extraction/theories/Erasure.v
@@ -1,6 +1,8 @@
 From Coq Require Import Bool.
 From Coq Require Import List.
 From Coq Require Import String.
+From Coq Require VectorDef.
+From Coq Require Import Psatz.
 From Equations Require Import Equations.
 From MetaCoq.Erasure Require Import EArities.
 From MetaCoq.Erasure Require Import Extract.
@@ -11,7 +13,9 @@ From MetaCoq.PCUIC Require Import PCUICAstUtils.
 From MetaCoq.PCUIC Require Import PCUICConfluence.
 From MetaCoq.PCUIC Require Import PCUICCumulativity.
 From MetaCoq.PCUIC Require Import PCUICElimination.
+From MetaCoq.PCUIC Require Import PCUICGeneration.
 From MetaCoq.PCUIC Require Import PCUICInversion.
+From MetaCoq.PCUIC Require Import PCUICNormal.
 From MetaCoq.PCUIC Require Import PCUICPrincipality.
 From MetaCoq.PCUIC Require Import PCUICSN.
 From MetaCoq.PCUIC Require Import PCUICSR.
@@ -30,18 +34,106 @@ Import ListNotations.
 Import MonadNotation.
 Set Equations Transparent.
 
-Section fix_sigma.
+Module P := PCUICAst.
+
+Section FixSigma.
 Local Existing Instance extraction_checker_flags.
 Context (Σ : global_env_ext).
 Context (wfextΣ : ∥wf_ext Σ∥).
 Let wfΣ : ∥wf Σ∥ := ltac:(now sq).
 
+
 Notation term_rel := (SafeErasureFunction.term_rel Σ).
 Instance WellFounded_term_rel : WellFounded term_rel :=
   (SafeErasureFunction.wf_reduction Σ wfΣ).
 
-Check (fun X : Type => X).
-(* Flag of a term indexed by the term's type. For example, for
+Inductive term_sub_ctx : context * term -> context * term -> Prop :=
+| sub_prod_dom Γ na A B : term_sub_ctx (Γ, A) (Γ, tProd na A B)
+| sub_prod_cod Γ na A B : term_sub_ctx (Γ,, vass na A, B) (Γ, tProd na A B)
+| sub_app_arg Γ arg hd arg1 :
+    In arg (decompose_app (tApp hd arg1)).2 ->
+    term_sub_ctx (Γ, arg) (Γ, tApp hd arg1).
+
+(*
+Instance WellFounded_term_sub_ctx : WellFounded term_sub_ctx.
+Proof.
+  Admitted.
+  intros (Γl & tl).
+  revert Γl.
+  induction tl; intros Γl; constructor; intros (Γs & ts) sub; inversion sub; subst; auto.
+  cbn in *.
+  revert ts sub H0.
+  induction (decompose_app_rec tl1 [tl2]).2 eqn:eq using List.rev_ind; [easy|].
+  intros ts sub H0.
+  SearchAbout (In _ (_ ++ _)).
+  apply in_app_or in H0.
+  destruct H0.
+  - admit.
+  - cbn in H.
+    destruct H as [->|[]].
+    replace ts with tl2; [easy|].
+    clear -eq.
+    assert (forall (l : list term) a b, [a] = (l ++ [b])%list -> a = b).
+    { intros.
+      replace l0 with (@nil term) in *.
+      - cbn in *.
+        now inversion H.
+      - symmetry. apply length_zero_iff_nil.
+        assert (List.length (l0 ++ [b]) = 1) by (now rewrite <- H).
+        rewrite List.app_length in H0.
+        cbn in H0.
+        lia.
+    }
+    induction tl1; cbn in *; try solve [now apply H with l].
+    clear H.
+    destruct l; [inversion eq; auto|].
+    inversion eq.
+    inversion H1.
+  apply app_in in H0.
+  destruct H0.
+  - subst.
+    SearchAbout decompose_app_rec.
+  - inversion sub.
+*)
+
+(*
+Instance foo : WellFounded term_direct_sub_ctx.
+Proof.
+  intros tl.
+  induction tl; try solve [constructor; intros ? sub; inversion sub; auto].
+  - constructor.
+    intros y sub.
+    inversion sub; subst; clear sub; auto.
+  - constructor.
+    intros
+  constructor.
+  induction tl; intros ts sub; try solve [inversion sub].
+  - inversion sub; subst; clear sub.
+    +
+  -
+*)
+
+Definition erase_type_rel : Relation_Definitions.relation (∑ Γ t, ∥isType Σ Γ t∥) :=
+  fun '(Γs; ts; wfs) '(Γl; tl; wfl) =>
+    ∥∑r, red Σ Γl tl r × term_sub_ctx (Γs, ts) (Γl, r)∥.
+
+Instance WellFounded_erase_type_rel : WellFounded erase_type_rel.
+Proof.
+  Admitted.
+(*
+  intros (Γl & l & wf).
+  sq.
+  induction (normalisation' _ _ _ wfΣ wf) as [l _ IH].
+  induction (WellFounded_term_sub_ctx (Γl, l)) as [? _ IH_sub] in Γl, wf, IH.
+  constructor.
+  intros (Γs & s & wfs) [(m & redm & sub)].
+  inversion sub; subst; clear sub.
+*)
+
+Definition Is_conv_to_Sort Γ T : Prop :=
+  exists univ, ∥red Σ Γ T (tSort univ)∥.
+
+(* type_flag of a term indexed by the term's type. For example, for
       t    :   T
    eq_refl : 5 = 5 : Prop
    we would pass T to flag_of_type below, and it would give
@@ -49,16 +141,19 @@ Check (fun X : Type => X).
    (fun (X : Type) => X) : Type -> Type
    we would pass Type -> Type and get is_logical = false, is_arity = true.
 *)
-Record Flag {Γ T} :=
+Record type_flag {Γ T} :=
   build_flag
-    { (* Term is a proof when fully applied, i.e. either
-         (t : T : Prop, or t a0 .. an : Prop) *)
+    { (* Type is proposition when fully applied, i.e. either
+         (T : Prop, or T a0 .. an : Prop) *)
       is_logical : bool;
-      (* Term is a type scheme, i.e. T = SProp/Type/Prop or iterated product *)
+      (* Term is a type scheme, i.e. type is an arity.
+         T = SProp/Type/Prop or ... -> SProp/Type/Prop *)
       is_arity : {Is_conv_to_Arity Σ Γ T} + {~Is_conv_to_Arity Σ Γ T};
+      (* Term is a type, i.e. type is a sort. *)
+      is_sort : {Is_conv_to_Sort Γ T} + {~Is_conv_to_Sort Γ T};
     }.
 
-Global Arguments Flag : clear implicits.
+Global Arguments type_flag : clear implicits.
 
 Lemma sq_red_transitivity {Γ A} B {C} :
   ∥red Σ Γ A B∥ ->
@@ -100,63 +195,60 @@ fot_discr (tProd _ _ _) := False;
 fot_discr (tSort _) := False;
 fot_discr _ := True.
 
-Inductive FotView : term -> Type :=
-| fot_view_prod na A B : FotView (tProd na A B)
-| fot_view_sort univ : FotView (tSort univ)
-| fot_view_other t : fot_discr t -> FotView t.
+Inductive fot_view : term -> Type :=
+| fot_view_prod na A B : fot_view (tProd na A B)
+| fot_view_sort univ : fot_view (tSort univ)
+| fot_view_other t : fot_discr t -> fot_view t.
 
-Equations fot_viewc (t : term) : FotView t :=
+Equations fot_viewc (t : term) : fot_view t :=
 fot_viewc (tProd na A B) := fot_view_prod na A B;
 fot_viewc (tSort univ) := fot_view_sort univ;
 fot_viewc t := fot_view_other t _.
 
+Lemma isTwf {Γ T} (isT : ∥isType Σ Γ T∥) : wellformed Σ Γ T.
+Proof. sq. now apply isType_wellformed. Qed.
+
 Opaque SafeErasureFunction.wf_reduction.
-Equations flag_of_type
-          (Γ : context) (wfΓ : ∥wf_local Σ Γ∥)
-          (T : term) (wtT : welltyped Σ Γ T)
-  : typing_result (Flag Γ T)
-  by wf ((Γ;T; or_introl wtT) : (∑ Γ t, wellformed Σ Γ t)) term_rel :=
-flag_of_type Γ wfΓ T wtT with inspect (hnf wfΣ Γ T (or_introl wtT)) :=
+Equations flag_of_type (Γ : context) (T : term) (isT : ∥isType Σ Γ T∥) : typing_result (type_flag Γ T)
+  by wf ((Γ;T; (isTwf isT)) : (∑ Γ t, wellformed Σ Γ t)) term_rel :=
+flag_of_type Γ T isT with inspect (hnf wfΣ Γ T (isTwf isT)) :=
   | exist T is_hnf with fot_viewc T := {
-    | fot_view_prod na A B with flag_of_type (Γ,, vass na A) _ B _ := {
+    | fot_view_prod na A B with flag_of_type (Γ,, vass na A) B _ := {
       | Checked flag_cod := ret {| is_logical := is_logical flag_cod;
-                                   is_arity := _ |};
+                                   is_arity := _ ;
+                                   is_sort := right _ |};
       | TypeError t := TypeError t
       };
     | fot_view_sort univ := ret {| is_logical := Universe.is_prop univ;
-                                   is_arity := left _; |};
+                                   is_arity := left _;
+                                   is_sort := left _; |};
     | fot_view_other T discr with type_of Σ wfΣ _ Γ T _ := {
       | Checked (existT _ K typK) with reduce_to_sort wfΣ Γ K _ := {
-        | Checked (existT _ univ _) :=
+        | Checked (existT _ univ red_univ) :=
           ret {| is_logical := Universe.is_prop univ;
-                 is_arity := right _; |};
+                 is_arity := right _;
+                 is_sort := right _; |};
         | TypeError t := TypeError t
         };
       | TypeError t := TypeError t
       }
     }.
 Next Obligation.
-  pose proof (@hnf_sound _ _ wfΣ Γ T (or_introl wtT)) as [sound].
-  rewrite <- is_hnf in sound.
-  assert (wt: welltyped Σ Γ (tProd na A B)) by (eapply red_welltyped; easy).
-  destruct wt as [? typ].
-  destruct wfΣ.
-  apply inversion_Prod in typ as (s & _ & Hs & _); [|easy].
-  now sq; apply wf_local_vass with s.
+  pose proof (@hnf_sound _ _ wfΣ _ _ (isTwf isT)) as [red_hnf].
+  destruct isT as [[univ typ]].
+  destruct wfΣ as [wfΣu].
+  assert (prod_ty: Σ;;; Γ |- tProd na A B : tSort univ).
+  { apply subject_reduction with T; [easy|easy|].
+    rewrite is_hnf.
+    apply red_hnf. }
+  apply inversion_Prod in prod_ty; [|easy].
+  destruct prod_ty as (? & s & ? & ? & ?).
+  constructor.
+  exists s.
+  easy.
 Qed.
 Next Obligation.
-  enough (wtprod: welltyped Σ Γ (tProd na A B)).
-  { destruct wtprod as [? wtprod].
-    destruct wfΣ.
-    apply inversion_Prod in wtprod as (? & ? & ? & ? & ?); [|easy].
-    econstructor.
-    easy. }
-  rewrite is_hnf.
-  apply red_welltyped with T; [easy|easy|].
-  apply hnf_sound.
-Qed.
-Next Obligation.
-  pose proof (@hnf_sound _ _ wfΣ Γ T (or_introl wtT)) as [sound].
+  pose proof (@hnf_sound _ _ wfΣ Γ T (isTwf isT)) as [sound].
   sq.
   exists na, A.
   rewrite is_hnf.
@@ -178,19 +270,629 @@ Next Obligation.
     { eapply Is_conv_to_Arity_red with T; [easy|].
       rewrite is_hnf.
       apply hnf_sound. }
-
     destruct prod_conv as [tm [[redtm] ar]].
     destruct wfΣ.
     apply invert_red_prod in redtm; [|easy].
     destruct redtm as (A' & B' & (-> & redAA') & redBB').
     exists B'; easy.
 Qed.
+Next Obligation.
+  destruct H as [univ [red_sort]].
+  pose proof (@hnf_sound _ _ wfΣ Γ T (isTwf isT)) as [red_prod].
+  rewrite <- is_hnf in red_prod.
+  destruct wfΣ as [wfΣu].
+  pose proof (red_confluence wfΣu red_sort red_prod) as (v' & redv'1 & redv'2).
+  apply invert_red_sort in redv'1.
+  subst.
+  apply invert_red_prod in redv'2 as (? & ? & (? & ?) & ?); easy.
+Qed.
+Next Obligation.
+  exists (tSort univ).
+  split; [|easy].
+  rewrite is_hnf.
+  apply hnf_sound.
+Qed.
+Next Obligation.
+  exists univ.
+  rewrite is_hnf.
+  apply hnf_sound.
+Qed.
+Next Obligation.
+  case wfextΣ.
+  now intros [].
+Qed.
+Next Obligation.
+  destruct isT as [[]].
+  now econstructor.
+Qed.
+Next Obligation.
+  sq.
+  apply typing_wellformed with T; [easy| |easy].
+  now case wfextΣ; intros [].
+Qed.
+Next Obligation.
+  (* We need to show that T is not convertible to an arity under
+     the assumption that hnf of T is neither tProd nor tSort.
+     To do this we will need to use some completeness fact about hnf,
+     which is not proved in MetaCoq yet, so we defer this proof for now. *)
+  destruct wfΣ as [wfΣu].
+  apply Is_conv_to_Arity_inv in H; [|easy].
+  Admitted.
+Next Obligation.
+  (* Like above, but we need to short that T is not converible to a sort. *)
+  Admitted.
 
-Lemma is_type_scheme_spec Γ wfΓ T wtT f :
-  flag_of_type Γ wfΓ T wtT = Checked f ->
-  is_type_scheme f ->
-  {Is_conv_to_Arity Σ Γ T} + {~Is_conv_to_Arity Σ Γ T}.
+(** OCaml-like types with boxes *)
+Inductive box_type :=
+| TBox
+| TAny
+| TArr (dom : box_type) (codom : box_type)
+| TApp (_ : box_type) (_ : box_type)
+| TVar (_ : nat) (* Index of type variable *)
+| TInd (_ : inductive)
+| TConst (_ : ident).
+
+Definition isTypeScheme (Γ : context) (t : term) : Type :=
+  ∑ (T : term), (Σ;;;Γ |- t : T) * (Is_conv_to_Arity Σ Γ T).
+
+Inductive eraset_input :=
+| et_type (Γ : context)
+          (t : term)
+          (args : list term)
+          (isT : ∥isType Σ Γ (mkApps t args)∥)
+          (var_map : Vector.t nat (List.length Γ)) (* tRel to TVar map *)
+(* Erase a type scheme (which can be nullary, i.e. just a type).
+   Note that this eta expands type schemes so they are always fully applied.
+   For example, [option] in [Definition foo := option.] is erased to
+   [([var1], TApp (TInd "option") (TVar 0))]. *)
+| et_type_scheme (Γ : context)
+                 (t : term)
+                 (isTS : ∥isTypeScheme Γ t∥).
+
+Definition redβιζ : RedFlags.t :=
+  {| RedFlags.beta := true;
+     RedFlags.iota := true;
+     RedFlags.zeta := true;
+     RedFlags.delta := false;
+     RedFlags.fix_ := true;
+     RedFlags.cofix_ := true |}.
+
+Import VectorDef.VectorNotations.
+Open Scope list.
+  (*
+  intros (Γl & l & wf).
+  sq.
+  induction (normalisation' _ _ _ wfΣ wf) as [l _ IH].
+  induction (well_founded_term_subterm l) as [l _ IH_sub] in Γl, wf, IH.
+  constructor.
+  intros (Γs & s & wfs) [(m & redm & sub)].
+  induction sub.
+  - admit.
+  - apply IHsub1.
+  inversion redm; subst; clear redm.
+  - apply IH_sub; [easy|].
+    induction (normalisation' _ _ _ wfΣ wf) as [? _ ?].
+  - clear IH_sub.
+    induction sub.
+    + inversion H; subst; clear H.
+      *
+    induction (normalisation' _ _ _ wfΣ wfs).
+
+    unfold WellFounded, well_founded in H.
+  induction sub.
+  - inversion H; subst; clear H.
+    +
+  assert (wellformed Σ Γl m).
+  { now apply red_wellformed with l. }
+  enough (Acc erase_type_rel (Γl; m; H)).
+  {
+  intros (Γm & m & isTm) [(super & redsuper & sub)].
+  inversion sub; subst; clear sub.
+  - inversion H; subst; clear H.
+    + inversion redsuper; subst; clear redsuper.
+      *
+      apply
+  induction sub.
+  - inversion H; subst; clear H.
+    +
+  specialize (IH super _).
+*)
+
+Fixpoint mk_apps_bt (t : box_type) (l : list box_type) :=
+  match l with
+  | [] => t
+  | u :: l' => mk_apps_bt (TApp t u) l'
+  end.
+
+Definition app_argsM {T : Type -> Type} `{Monad T} {A} (f : P.term -> T A) :=
+  fix go (t : P.term) :=
+    match t with
+    | P.tApp t1 t2 =>
+      hd <- f t2 ;;
+      tl <- go t1 ;;
+      ret (hd :: tl)
+    | _ => ret []
+    end.
+
+Definition check_tvars_empty (tvars : list name) (t : term) : typing_result unit :=
+  match tvars with
+  | [] => ret tt
+  | _ => TypeError (Msg ("Unsupported type " ++ string_of_term t))
+  end.
+
+(*
+(* A check_isType that uses retyping *)
+Program Definition check_isType Γ t (wt : welltyped Σ Γ t) : typing_result (∥isType Σ Γ t∥) :=
+  '(ty; typ) <- type_of Σ wfΣ _ Γ t wt;;
+  '(univ; red) <- reduce_to_sort wfΣ Γ ty _;;
+  ret _.
+Next Obligation.
+  now destruct wfextΣ as [[]].
+Qed.
+Next Obligation.
+  sq.
+  apply typing_wellformed with t.
+  - easy.
+  - now destruct wfextΣ as [[]].
+  - easy.
+Qed.
+Next Obligation.
+  sq.
+  exists x.
+  eapply type_reduction; try easy.
+  eapply typing_wf_local; easy.
+Qed.
+*)
+
+Lemma reduce_term_sr {Γ t red wft s} :
+  s = reduce_term red Σ wfΣ Γ t wft ->
+  ∥isType Σ Γ t∥ ->
+  ∥isType Σ Γ s∥.
 Proof.
-  intros checks ts.
-  funelim (flag_of_type Γ wfΓ T wtT).
-  -
+  intros -> [(univ & ?)].
+  pose proof (reduce_term_sound red Σ wfΣ Γ t wft) as [redt].
+  destruct wfΣ as [wfΣu].
+  constructor.
+  exists univ.
+  now apply subject_reduction with t.
+Qed.
+
+Lemma decompose_app_rec_acc_app_full t l l' :
+  (decompose_app_rec t (l ++ l')).2 = (decompose_app_rec t l).2 ++ l'.
+Proof.
+  revert l l'.
+  induction t; try easy.
+  intros l l'.
+  cbn.
+  now rewrite app_comm_cons.
+Qed.
+
+Lemma decompose_app_rec_acc_app t l :
+  (decompose_app_rec t l).2 = (decompose_app_rec t []).2 ++ l.
+Proof.
+  apply (decompose_app_rec_acc_app_full _ [] l).
+Qed.
+
+Definition erase_app_head (t : term) : typing_result box_type :=
+  match t with
+  | tConst nm _ => ret (TConst nm)
+  | tInd ind _ => ret (TInd ind)
+  | _ => TypeError (Msg ("Unsupported head in decomposed application "
+                           ++ string_of_term t))
+  end.
+
+Fixpoint mkApps_bt (head : box_type) (l : list box_type) : box_type :=
+  match l with
+  | [] => head
+  | x :: xs => mkApps_bt (TApp head x) xs
+  end.
+
+Equations erase_type_discr (t : term) : Prop := {
+  | tRel _ := False;
+  | tSort _ := False;
+  | tProd _ _ _ := False;
+  | tApp _ _ := False;
+  | tConst _ _ := False;
+  | tInd _ _ := False;
+  | _ := True
+  }.
+
+Inductive erase_type_view : term -> Type :=
+| et_view_rel i : erase_type_view (tRel i)
+| et_view_sort u : erase_type_view (tSort u)
+| et_view_prod na A B : erase_type_view (tProd na A B)
+| et_view_app hd arg : erase_type_view (tApp hd arg)
+| et_view_const kn u : erase_type_view (tConst kn u)
+| et_view_ind ind u : erase_type_view (tInd ind u)
+| et_view_other t : erase_type_discr t -> erase_type_view t.
+
+Equations erase_type_viewc (t : term) : erase_type_view t := {
+  | tRel i := et_view_rel i;
+  | tSort u := et_view_sort u;
+  | tProd na A B := et_view_prod na A B;
+  | tApp hd arg := et_view_app hd arg;
+  | tConst kn u := et_view_const kn u;
+  | tInd ind u := et_view_ind ind u;
+  | t := et_view_other t _
+  }.
+
+Equations erase_type
+          (Γ : context)
+          (t : term)
+          (isT : ∥isType Σ Γ t∥)
+          (var_map : Vector.t nat (List.length Γ)) (* tRel to TVar map *)
+  : typing_result (list name × box_type)
+  by wf ((Γ; t; isT) : (∑ Γ t, ∥isType Σ Γ t∥)) erase_type_rel :=
+erase_type Γ t isT var_map with inspect (reduce_term redβιζ Σ wfΣ Γ t (isTwf isT)) :=
+  (* matching on flag_of_type directly causes issues for some reason *)
+  | exist thnf eq_hnf with flag_of_type Γ thnf _ := {
+    | TypeError te := TypeError te;
+
+    | Checked {| is_logical := true |} := ret ([], TBox);
+
+    | Checked _ with erase_type_viewc thnf := {
+
+      | et_view_rel i := ret ([], TVar (@Vector.nth_order _ _ var_map i _));
+
+      | et_view_sort _ := ret ([], TBox);
+
+      | et_view_prod na A B with erase_type Γ A _ var_map := {
+        | TypeError te := TypeError te;
+
+        | Checked ([], dom) with erase_type (Γ,, vass na A) B _ (0 :: var_map)%vector := {
+          | TypeError te := TypeError te;
+          | Checked (tvars, cod) := ret (na :: tvars, TArr dom cod)
+          };
+
+        | Checked _ := TypeError (Msg "Type is not in prenex form")
+        };
+
+      | et_view_app orig_hd orig_arg with inspect (decompose_app (tApp orig_hd orig_arg)) := {
+        | exist (hd, decomp_args) _ with erase_app_head hd := {
+          | TypeError te := TypeError te;
+
+          | Checked hdbt :=
+
+            let erase_arg (a : term) (i : In a decomp_args) : typing_result box_type :=
+                '(aT; typ) <- type_of Σ wfΣ _ Γ a _;;
+                ft <- flag_of_type Γ aT isTy;;
+                match ft with
+                | {| is_logical := true |} => ret TBox
+                | {| is_sort := left _ |} =>
+                  '(tvars, bt) <- erase_type Γ a _ var_map;;
+                  match tvars with
+                  | [] => ret bt
+                  | _ => TypeError (Msg ("Type is not in prenex form"))
+                  end
+                | _ =>
+                  TypeError (Msg ("Cannot erase argument; "
+                                    ++ "it is not a type or logical type scheme "
+                                    ++ string_of_term a))
+                end in
+
+            (fix erase_args
+                 (args : list term) (inc : incl args decomp_args)
+                 (result : box_type) : typing_result (list name * box_type) :=
+               match args with
+               | [] => ret ([], result)
+               | a :: args =>
+                 abt <- erase_arg a _;;
+                 erase_args args _ (TApp result abt)
+               end) decomp_args _ hdbt
+
+          (* The code below gives a weird error *)
+          (*
+          where erase_args (args : list term) (inc : incl args decomp_args)
+                : typing_result (list box_type) :=
+          erase_args [] _ := ret [];
+          (* We will fail if the arg is not a type, but let's first check to see if
+             it is a logical type scheme, in which case we can get away with boxing
+             it. For instance: Say we are processing [sig A P] in
+               A : Type, P : A -> Prop |- sig A P : Type.
+             The P argument here is not strictly a type, but is rather a type scheme.
+             So we get the flag of its type, and box it. *)
+          erase_args (a :: args) _ := abt <- erase_arg a _;;
+                                      argsbt <- erase_args args _;;
+                                      ret (abt :: argsbt)
+
+          where erase_arg (a : term) (i : In a decomp_args) : typing_result box_type :=
+          erase_arg a i with type_of Σ wfΣ _ Γ a _ := {
+            | TypeError te := TypeError te;
+            | Checked (aT; typ) with flag_of_type Γ aT _ := {
+              | TypeError te := TypeError te;
+              | Checked {| is_logical := true |} := ret TBox;
+              (* If aT is a sort, then a is a type, so continue erasing it *)
+              | Checked {| is_sort := left _ |} with erase_type Γ a _ var_map := {
+                | TypeError te := TypeError te;
+                | Checked ([], bt) := ret bt;
+                | Checked _ := TypeError (Msg ("Type is not in prenex form"))
+                };
+
+              | Checked _ := TypeError (Msg ("Cannot erase argument; "
+                                               ++ "it is not a type or logical type scheme "
+                                               ++ string_of_term a))
+              }
+            }
+          *)
+          }
+        };
+
+      | et_view_const kn _ := ret ([], TConst kn);
+
+      | et_view_ind ind _ := ret ([], TInd ind);
+
+      | et_view_other t _ := TypeError (Msg ("Unsupported type "
+                                               ++ string_of_term t))
+
+      }
+  }.
+Next Obligation.
+  now eapply reduce_term_sr.
+Qed.
+Next Obligation.
+  pose proof (reduce_term_sr eq_hnf isT) as [(univ & typ)].
+  destruct wfΣ as [wfΣu].
+  apply inversion_Rel in typ; [|easy].
+  apply nth_error_Some.
+  destruct typ as (? & _ & ? & _).
+  congruence.
+Qed.
+Next Obligation.
+  pose proof (reduce_term_sr eq_hnf isT) as [(univ & typ)].
+  destruct wfΣ as [wfΣu].
+  apply inversion_Prod in typ; [|easy].
+  destruct typ as (s1 & _ & ? & _ & _).
+  sq.
+  now exists s1.
+Qed.
+Next Obligation.
+  pose proof (reduce_term_sound redβιζ Σ wfΣ Γ t (isTwf isT)) as [red].
+  sq.
+  exists (tProd na A B).
+  split; [rewrite eq_hnf; easy|].
+  constructor.
+Qed.
+Next Obligation.
+  pose proof (reduce_term_sr eq_hnf isT) as [(univ & typ)].
+  destruct wfΣ as [wfΣu].
+  apply inversion_Prod in typ; [|easy].
+  destruct typ as (s1 & s2 & ? & ? & _).
+  sq.
+  now exists s2.
+Qed.
+Next Obligation.
+  pose proof (reduce_term_sound redβιζ Σ wfΣ Γ t (isTwf isT)) as [red].
+  sq.
+  exists (tProd na A B).
+  split; [rewrite eq_hnf; easy|].
+  constructor.
+Qed.
+Next Obligation.
+  now case wfextΣ; intros [[]].
+Qed.
+Next Obligation.
+  Admitted.
+Next Obligation.
+  destruct typ as [typ].
+  apply validity_term in typ.
+  SearchAbout welltyped.
+  SearchAbout (tSort _).
+  SearchAbout validity.
+  SearchAbout Is_conv_to_Arity.
+Next Obligation.
+  pose proof (reduce_term_sound redβιζ Σ wfΣ Γ t (isTwf isT)).
+  sq.
+  exists (tApp hd0 arg).
+  split.
+  - now rewrite wildcard.
+  - constructor.
+    cbn.
+    rewrite decompose_app_rec_acc_app.
+    now apply in_or_app; right; constructor.
+Qed.
+
+    exist (tRel i) _ _ := Checked ([], TVar (@Vector.nth_order _ _ var_map i _));
+    erase
+
+  | exist (tRel i) _ := Checked ([], TVar (@Vector.nth_order _ _ var_map i _));
+  | exist (tSort _) _ := Checked ([], TBox);
+  | exist (tProd na A B) _ with flag_of_type Γ A _ := {
+    | Checked {| is_logical := false; is_arity := right _ |}
+      (* Domain is a simple type (like [nat]), erase codomain first. *)
+      with erase_type (Γ,, vass na A) B _ (0 :: var_map)%vector) := {
+      | Checked (tvars, TBox) := Checked (tvars, TBox)
+  }.
+
+
+
+
+Equations eraset (input : eraset_input)
+  : typing_result (list name × box_type)
+  by wf input eraset_input_rel :=
+eraset (et_type Γ t args isT var_map)
+  with inspect (reduce_term redβιζ Σ wfΣ Γ t _) := {
+  | exist (tRel i) _ := Checked ([], TVar (@Vector.nth_order _ _ var_map i _));
+  | exist (tApp hd arg) _ := eraset (et_type Γ hd (arg :: args) _ var_map);
+  | exist (tSort _) _ := Checked ([], TBox);
+  | exist (tProd na A B) _ with flag_of_type Γ A _ := {
+    | Checked {| is_logical := false; is_arity := right _ |}
+      (* domain is a simple type like nat, erase codomain first *)
+      with eraset (et_type (Γ,, vass na A) B [] _ (0 :: var_map)%vector) := {
+      | Checked (tvars, TBox) := Checked (tvars, TBox);
+      | Checked (tvars, cod) with eraset (et_type Γ A [] _ var_map) := {
+        | Checked ([], dom) := Checked (tvars, TArr dom cod);
+        | Checked _ := TypeError (Msg "Type is not in prenex normal form");
+        | TypeError m := TypeError m
+        };
+      | TypeError m := TypeError m
+      };
+    | _ := todo "rest"
+    };
+  | exist _ _ := todo "rest"
+  };
+eraset (et_type_scheme Γ t isTS) := todo "rest".
+
+
+(* Erase the type (mkApps t args). *)
+Equations erase_type
+          (Γ : context)
+          (t : term)
+          (args : list term)
+          (isT : ∥isType Σ Γ (mkApps t args)∥)
+          (var_map : Vector.t nat (length Γ)) (* TRel to TVar map *)
+          (names : list name)
+  : typing_result (list name * box_type) :=
+erase_type Γ t args isT with inspect (reduce_term red_beta_iota_zeta wfΣ Γ t _) := {
+  | exist (tRel i) _ := TVar (@Vector.nth_order _ _ var_map i _);
+  | exist (tApp head arg) _ := erase_type Γ head (arg :: args) _ var_map names;
+  | exist (tSort _) _ := TBox;
+  | exist (tProd na A B) _ with flag_of_type Γ A _ := {
+    | Checked f
+
+(* Erase the type (mkApps t args) *)
+where aux (Γ : context) (t : term) (args : list term) (isT : ∥isType Σ Γ (mkApps t args)∥)
+         : typing_result (list name * box_type) :=
+aux Γ t args isT with inspect (hnf
+
+Lemma isTSwf {Γ t} (isTS : ∥isTypeScheme Γ t∥) : wellformed Σ Γ t.
+Proof.
+  destruct isTS as [[]].
+  left.
+  now econstructor.
+Qed.
+
+(* Erase a type scheme (which can be nullary, i.e. just a type).
+   Note that this eta expands type schemes so they are always fully applied.
+   For example, [option] in [Definition foo := option.] is erased to
+   [([var1], TApp (TInd "option") (TVar 0))]. *)
+Equations erase_type_scheme
+          (Γ : context)
+          (t : term)
+          (isTS : ∥isTypeScheme Γ t∥) : typing_result (list name * box_type) :=
+erase_type_scheme Γ t isTS with inspect (hnf Σ wfΣ Γ t (isTSwf isTS)) := {
+  | exist (tApp head arg) _ with erase_type_scheme Γ head _ := {
+    | Checked ((nahd :: natl), head) :=
+
+Inductive eraset_input :=
+| eraset_type (Γ : context)
+              (t : term)
+              (args : list term)
+              (isT : ∥isType Σ Γ (mkApps t args)∥)
+(* Erase a type scheme (which can be nullary, i.e. just a type).
+   Note that this eta expands type schemes so they are always fully applied.
+   For example, [option] in [Definition foo := option.] is erased to
+   [([var1], TApp (TInd "option") (TVar 0))]. *)
+| eraset_type_scheme (Γ : context)
+                     (t : term)
+                     (isTS : ∥isTypeScheme Γ t∥).
+
+
+Equations erase_type_scheme
+
+
+Equations eraset (input : eraset_input) : typing_result (list name * box_type)
+
+Equations erase_type_scheme
+          (Γ : context)
+          (t : term)
+          (isTS : ∥isTypeScheme Γ t∥) : typing_result (list name * box_type) :=
+erase_type_scheme
+
+Axiom actually_isType : forall {Γ ty} (wt : welltyped Σ Γ ty), ∥isType Σ Γ ty∥.
+
+(** The type erasure procedure. It produces a list of names used to bind type variables and a prenex type with some parts (corresponding to quantification over types and propositions) replaced with boxes. Fails for types that are not prenex or non-extractable dependent types (e.g. containing constructors of inductive types) *)
+Program Fixpoint erase_type
+           (Γ : context)
+           (db : list (option nat)) (* for reindexing tRels in types *)
+           (names : list name) (* names of the binders in [tProd] for further printing *)
+           (j : nat) (* how many binders we are under *)
+           (l_arr : bool) (* [true] is we are erasing a domain of the function type*)
+           (ty : P.term)
+           (* TODO: we need to pass [isType] instead, but this requires to
+             implement the function in a different way *)
+           (Hty : welltyped Σ Γ ty)
+  : typing_result (list name * box_type) :=
+  match flag_of_type Γ ty (actually_isType Hty) with
+  | Checked (Some r) => ret (names, TBox r)
+  | TypeError (NotASort _) (* TODO: figure out how to get rid of this case*)
+  | Checked None =>
+    match ty with
+    | P.tRel i =>
+      (* we use well-typedness to provide a witness that there is something in the context *)
+      let v := safe_nth Γ (exist i _) in
+      match (nth_error db i) with
+      | Some (Some n) => ret (names, TVar n)
+      | Some None => TypeError (Msg ("Variable " ++ string_of_name v.(decl_name) ++ " is not translated. Probably not a prenex type"))
+      | _ => TypeError (Msg ("Variable " ++ string_of_name v.(decl_name) ++ " is not found in the translation context"))
+      end
+    | P.tSort _ => ret (names,TBox E.ER_type)
+    | P.tProd na t b =>
+      let wt_t := _ in
+      let wt_b := _ in
+      ft <- flag_of_type Γ t wt_t ;;
+      match flag_of_type (P.vass na t :: Γ) b wt_b with
+          | Checked (Some _) => ret (names, TBox E.ER_type)
+          | Checked None =>
+            (* we pass [true] flag to indicate that we translate the domain *)
+            '(nms1, t1) <- erase_type Γ db names j true t wt_t ;;
+            (* if it is a binder for a type variable, e.g [forall A, ...] and we are in the codomain, we add current variable to the translation context [db], otherwise, we add [None], because it's either not a binder for a type variable or the type is not prenex. This guarantees that non-prenex types will fail *)
+            let db' := if is_arity ft && (negb l_arr) then Some j :: db
+                       else None :: db in
+            (* we only count binders for type variables *)
+            let j' := if is_arity ft then (1+j)%nat else j in
+            '(nms2, t2) <- erase_type (P.vass na t :: Γ) db' names j' l_arr b wt_b ;;
+            (* we keep track of the binders for types *)
+            let names' := if is_arity ft then (nms1++ [na] ++ nms2)%list
+                          else (nms1 ++ nms2)%list in
+            ret (names', TArr t1 t2)
+          | TypeError te => TypeError te
+      end
+    | P.tApp t1 t2 =>
+      '(nms1, t1') <- erase_type Γ db names j l_arr t1 _ ;;
+      '(nms2,t2') <- erase_type Γ db names j l_arr t2 _ ;;
+      ret (nms1 ++ nms2, TApp t1' t2')%list
+    | P.tInd ind _ =>
+      decl <- lookup_ind_decl ind ;;
+      let oib := projT1 (projT2 decl) in
+      ret (names,TInd ind)
+    | P.tLambda na t b => (* NOTE: assume that this is a type scheme, meaning that applied to enough args it ends up a type *)
+      erase_type (P.vass na t :: Γ) db names j l_arr b _
+    | P.tConst nm _ =>
+      (* NOTE: since the original term is well-typed (need also to be a type!), we know that the constant, applied to enough arguments is a valid type (meaning that the constant is a type scheme), so, we just leave the constant name in the erased version *)
+      ret (names, TConst nm)
+    | P.tEvar _ _  | P.tCase _ _ _ _ | P.tProj _ _
+    | P.tFix _ _ | P.tCoFix _ _ | P.tVar _ | P.tLetIn _ _ _ _
+    | P.tConstruct _ _ _ => TypeError (Msg ("Not supported type: " ++ string_of_term ty))
+    end
+  | TypeError te => TypeError te
+  end.
+Solve Obligations with
+    ((intros;subst;
+    try clear dependent filtered_var;
+    try clear dependent filtered_var0;
+    try clear dependent Heq_anonymous;
+     try clear dependent Heq_anonymous0);try solve_erase;try easy).
+Next Obligation.
+  sq'. inversion Hty as [? X]. eapply inversion_Rel in X as (? & ? & ? & ?);eauto.
+  apply nth_error_Some;easy.
+Qed.
+Next Obligation. easy. Qed.
+Next Obligation.
+  clear dependent Heq_anonymous;solve_erase.
+Qed.
+Next Obligation.
+  sq'. inversion Hty as [? X]. eapply inversion_Rel in X as (? & ? & ? & ?);eauto.
+  apply nth_error_Some;easy.
+Qed.
+Next Obligation. easy. Qed.
+Next Obligation.
+  clear dependent Heq_anonymous;solve_erase.
+Qed.
+
+Record one_inductive_body :=
+  {
+    ind_name : ident;
+    ind_type_parameters : list name;
+    ind_ctors : list (ident * list D.box_type);
+
+End FixSigma.
